src/HOL/Imperative_HOL/ex/Subarray.thy
@@ -30,20 +30,20 @@ by (simp add: sublist'_update3)
 lemma subarray_Nil: "n \<ge> m \<Longrightarrow> subarray n m a h = []"
 by (simp add: subarray_def sublist'_Nil')
 
-lemma subarray_single: "\<lbrakk> n < Array.length a h \<rbrakk> \<Longrightarrow> subarray n (Suc n) a h = [get_array a h ! n]" 
+lemma subarray_single: "\<lbrakk> n < Array.length h a \<rbrakk> \<Longrightarrow> subarray n (Suc n) a h = [get_array a h ! n]" 
 by (simp add: subarray_def length_def sublist'_single)
 
-lemma length_subarray: "m \<le> Array.length a h \<Longrightarrow> List.length (subarray n m a h) = m - n"
+lemma length_subarray: "m \<le> Array.length h a \<Longrightarrow> List.length (subarray n m a h) = m - n"
 by (simp add: subarray_def length_def length_sublist')
 
-lemma length_subarray_0: "m \<le> Array.length a h \<Longrightarrow> List.length (subarray 0 m a h) = m"
+lemma length_subarray_0: "m \<le> Array.length h a \<Longrightarrow> List.length (subarray 0 m a h) = m"
 by (simp add: length_subarray)
 
-lemma subarray_nth_array_Cons: "\<lbrakk> i < Array.length a h; i < j \<rbrakk> \<Longrightarrow> (get_array a h ! i) # subarray (Suc i) j a h = subarray i j a h"
+lemma subarray_nth_array_Cons: "\<lbrakk> i < Array.length h a; i < j \<rbrakk> \<Longrightarrow> (get_array a h ! i) # subarray (Suc i) j a h = subarray i j a h"
 unfolding Array.length_def subarray_def
 by (simp add: sublist'_front)
 
-lemma subarray_nth_array_back: "\<lbrakk> i < j; j \<le> Array.length a h\<rbrakk> \<Longrightarrow> subarray i j a h = subarray i (j - 1) a h @ [get_array a h ! (j - 1)]"
+lemma subarray_nth_array_back: "\<lbrakk> i < j; j \<le> Array.length h a\<rbrakk> \<Longrightarrow> subarray i j a h = subarray i (j - 1) a h @ [get_array a h ! (j - 1)]"
 unfolding Array.length_def subarray_def
 by (simp add: sublist'_back)
 
@@ -51,21 +51,21 @@ lemma subarray_append: "\<lbrakk> i < j; j < k \<rbrakk> \<Longrightarrow> subar
 unfolding subarray_def
 by (simp add: sublist'_append)
 
-lemma subarray_all: "subarray 0 (Array.length a h) a h = get_array a h"
+lemma subarray_all: "subarray 0 (Array.length h a) a h = get_array a h"
 unfolding Array.length_def subarray_def
 by (simp add: sublist'_all)
 
-lemma nth_subarray: "\<lbrakk> k < j - i; j \<le> Array.length a h \<rbrakk> \<Longrightarrow> subarray i j a h ! k = get_array a h ! (i + k)"
+lemma nth_subarray: "\<lbrakk> k < j - i; j \<le> Array.length h a \<rbrakk> \<Longrightarrow> subarray i j a h ! k = get_array a h ! (i + k)"
 unfolding Array.length_def subarray_def
 by (simp add: nth_sublist')
 
-lemma subarray_eq_samelength_iff: "Array.length a h = Array.length a h' \<Longrightarrow> (subarray i j a h = subarray i j a h') = (\<forall>i'. i \<le> i' \<and> i' < j \<longrightarrow> get_array a h ! i' = get_array a h' ! i')"
+lemma subarray_eq_samelength_iff: "Array.length h a = Array.length h' a \<Longrightarrow> (subarray i j a h = subarray i j a h') = (\<forall>i'. i \<le> i' \<and> i' < j \<longrightarrow> get_array a h ! i' = get_array a h' ! i')"
 unfolding Array.length_def subarray_def by (rule sublist'_eq_samelength_iff)
 
-lemma all_in_set_subarray_conv: "(\<forall>j. j \<in> set (subarray l r a h) \<longrightarrow> P j) = (\<forall>k. l \<le> k \<and> k < r \<and> k < Array.length a h \<longrightarrow> P (get_array a h ! k))"
+lemma all_in_set_subarray_conv: "(\<forall>j. j \<in> set (subarray l r a h) \<longrightarrow> P j) = (\<forall>k. l \<le> k \<and> k < r \<and> k < Array.length h a \<longrightarrow> P (get_array a h ! k))"
 unfolding subarray_def Array.length_def by (rule all_in_set_sublist'_conv)
 
-lemma ball_in_set_subarray_conv: "(\<forall>j \<in> set (subarray l r a h). P j) = (\<forall>k. l \<le> k \<and> k < r \<and> k < Array.length a h \<longrightarrow> P (get_array a h ! k))"
+lemma ball_in_set_subarray_conv: "(\<forall>j \<in> set (subarray l r a h). P j) = (\<forall>k. l \<le> k \<and> k < r \<and> k < Array.length h a \<longrightarrow> P (get_array a h ! k))"
 unfolding subarray_def Array.length_def by (rule ball_in_set_sublist'_conv)
 
 end
